src/Applicative_Examples.thy
@@ -3,8 +3,7 @@
 theory Applicative_Examples imports
   Applicative_Environment_Algebra
   Stream_Algebra
-  Tree_Traversal
-  Tree_Traversal2
+  Tree_Relabelling
 begin
 
 end
